Hoare_woc.v
@@ -45,14 +45,14 @@ Definition hoare_triple (fc : func_context) (lf : public_funcs) (P : Assertion) 
 
 Definition func_triple (fc : func_context) (lf : public_funcs) (P : Assertion) (f : func) (Q : Assertion) : Prop :=
   forall st1 st2,
-    ceval fc lf (snd (fc f)) st1 st2 ->
+    ceval fc lf (func_bdy f) st1 st2 ->
     P st1 ->
     Q st2.
 
 Notation "'|' fc ',' lf '|' '{{' P '}}' c '{{' Q '}}'" := (hoare_triple fc lf P c Q) (at level 90, c at next level).
 
 Definition pv_to_assertion (fc : func_context) (f : func) (pv : list aexp) (P : Assertion) : Assertion :=
-  fun st => P (param_to_local_state st (fst (fc f)) pv, snd st).
+  fun st => P (param_to_local_state st (func_arg f) pv, snd st).
 
 Theorem hoare_consequence : forall fc lf P P' Q Q' c,
   P |-- P' ->
